BPlusTree_ImpRange.thy
@@ -7,9 +7,72 @@ begin
 (* Adding an actual range iterator based on the normal iterator
 is trivial (just forward until we reach the first element \<ge> and stop
 as soon as we have an element <)
-We *could* implement a search for the first element of the range
-however cannot make any (simple) guarantees on its quality
-(see Bplustree_Range to see why *)
+We now try to implement a search for the first element of the range efficiently
+ *)
+subsection "The imperative split locale"
 
+locale imp_split_range = abs_split_range: split_range split lrange_list
+  for split::
+    "('a::{heap,default,linorder,order_top} bplustree \<times> 'a) list \<Rightarrow> 'a
+       \<Rightarrow> ('a bplustree \<times> 'a) list \<times> ('a bplustree \<times> 'a) list" 
+    and lrange_list ::  "'a \<Rightarrow> ('a::{heap,default,linorder,order_top}) list \<Rightarrow> 'a list" +
+  fixes imp_split:: "('a btnode ref option \<times> 'a::{heap,default,linorder,order_top}) pfarray \<Rightarrow> 'a \<Rightarrow> nat Heap"
+  assumes imp_split_rule [sep_heap_rules]:"sorted_less (separators ts) \<Longrightarrow>
+  length tsi = length rs \<Longrightarrow>
+  tsi'' = zip (zip (map fst tsi) (zip (butlast (r#rs)) (butlast (rs@[z])))) (map snd tsi) \<Longrightarrow>
+ <is_pfa c tsi (a,n) 
+  * blist_assn k ts tsi'' > 
+    imp_split (a,n) p 
+  <\<lambda>i. 
+    is_pfa c tsi (a,n)
+    * blist_assn k ts tsi''
+    * \<up>(split_relation ts (split ts p) i)>\<^sub>t"
+
+locale imp_split2 = abs_split_range: split_range split lrange_list + imp_split_range split lrange_list imp_split
+  for split::
+    "('a bplustree \<times> 'a::{heap,default,linorder,order_top}) list \<Rightarrow> 'a
+       \<Rightarrow> ('a bplustree \<times> 'a) list \<times> ('a bplustree \<times> 'a) list" 
+    and lrange_list ::  "'a \<Rightarrow> ('a::{heap,default,linorder,order_top}) list \<Rightarrow> 'a list"
+    and imp_split :: "('a btnode ref option \<times> 'a::{heap,default,linorder,order_top}) pfarray \<Rightarrow> 'a \<Rightarrow> nat Heap" +
+  fixes imp_lrange_list:: "'a \<Rightarrow> ('a::{heap,default,linorder,order_top}) pfarray \<Rightarrow> 'a pfa_it Heap"
+  assumes lrange_list_rule [sep_heap_rules]:"sorted_less ks \<Longrightarrow>
+   <is_pfa c ks (a',n')> 
+    imp_lrange_list x (a',n') 
+  <pfa_is_it c ks (a',n') (lrange_list x ks)>\<^sub>t"
+begin
+
+partial_function (heap) lrange_iter_init ::
+  "'a btnode ref \<Rightarrow> 'a \<Rightarrow> (('a btnode ref option \<times> 'a btnode ref option) \<times> 'a pfa_it option) Heap"
+  where
+    "lrange_iter_init p x = do {
+  node \<leftarrow> !p;
+  (case node of
+     Btleaf xs _ \<Rightarrow> do {
+        local_iter \<leftarrow> imp_lrange_list x xs;
+        return (((Some p,None),Some local_iter))
+      }
+       |
+     Btnode ts t \<Rightarrow> do {
+       i \<leftarrow> imp_split ts x;
+       tsl \<leftarrow> pfa_length ts;
+       if i < tsl then do {
+         s \<leftarrow> pfa_get ts i;
+         let (sub,sep) = s in
+           lrange_iter_init (the sub) x
+       } else
+           lrange_iter_init t x
+    }
+)}"
+
+(*TODO prove correct *)
+(* might need a modularization, where a z is inserted somewhere *)
+lemma lrange_iter_init_rule:
+  assumes "k > 0" "root_order k t"
+  shows "<bplustree_assn k t ti r None>
+lrange_iter_init ti x
+<\<lambda>it. leaf_elements_iter k t ti r (abs_split_range.lrange t x) it>\<^sub>t"
+  sorry
+
+end
 
 end
